DLean/USubst/Semantics.lean
@@ -333,11 +333,12 @@ theorem subst_adjoint_of_term_vector_to_subst
 
 theorem Subst.apply_subst_term_vector_to_term
   (σ : Subst)
+  (U : FCSet Assignable)
   {n : ℕ}
   (args a : TermVector n)
   (x : Fin n)
-  : TermVector.applySubst σ args = some a
-  → Term.applySubst σ args.toVector[x] = some a.toVector[x] := by
+  : TermVector.applySubst σ U args = some a
+  → Term.applySubst σ U args.toVector[x] = some a.toVector[x] := by
     intro h
     cases args with
       | nil => grind
@@ -395,9 +396,9 @@ theorem toSubst.freeVars_inc {n : ℕ} (args : TermVector n) (S : Option (Finset
 
 mutual
 
-theorem TermVector.freeVars_applySubst_subset {n : ℕ} (σ : Subst) (ts as : TermVector n)
-  : TermVector.applySubst σ ts = some as
-  → ↑as.freeVars ⊆ ↑ts.freeVars ∪ (σ.freeVars (some ts.signature)).toSet := by
+theorem TermVector.freeVars_applySubst_subset {n : ℕ} (σ : Subst) (U : FCSet Assignable) (ts as : TermVector n)
+  : TermVector.applySubst σ U ts = some as
+  → ↑as.freeVars ⊆ ↑ts.freeVars ∪ (σ.freeVars (some ts.signature) \ U).toSet := by
   intro h₁
   match n with
   | 0 =>
@@ -418,17 +419,17 @@ theorem TermVector.freeVars_applySubst_subset {n : ℕ} (σ : Subst) (ts as : Te
       clear h₁
       simp only [TermVector.freeVars_cons, Finset.coe_union, TermVector.signature_cons]
       have := @σ.freeVars_symbol_union t.signature ts'.signature
-      have := Term.freeVars_applySubst_subset σ t a heqa
-      have := TermVector.freeVars_applySubst_subset σ ts' as' heqas'
-      grind only [= Set.mem_union, = Set.subset_def]
+      have := Term.freeVars_applySubst_subset σ U t a heqa
+      have := TermVector.freeVars_applySubst_subset σ U ts' as' heqas'
+      grind only [= Set.subset_def, FCSet.to_set_diff, = Set.mem_union, = Set.mem_diff]
 termination_by (σ.size, sizeOf ts)
 decreasing_by
 all_goals simp_wf
 all_goals grind only [= Prod.lex_def]
 
-theorem Term.freeVars_applySubst_subset (σ : Subst) (t a : Term)
-  : Term.applySubst σ t = some a
-  → ↑a.freeVars ⊆ ↑t.freeVars ∪ (σ.freeVars (some t.signature)).toSet := by
+theorem Term.freeVars_applySubst_subset (σ : Subst) (U : FCSet Assignable) (t a : Term)
+  : Term.applySubst σ U t = some a
+  → ↑a.freeVars ⊆ ↑t.freeVars ∪ (σ.freeVars (some t.signature) \ U).toSet := by
   intro h₁
   match t with
   | .var v => simp_all[Term.applySubst]
@@ -437,7 +438,7 @@ theorem Term.freeVars_applySubst_subset (σ : Subst) (t a : Term)
     split at h₁
     . contradiction
     next a' heq =>
-    have := Term.freeVars_applySubst_subset σ t a' heq
+    have := Term.freeVars_applySubst_subset σ U t a' heq
     simp_all
     rw[← h₁]
     simp only[Term.freeVars, Term.signature]
@@ -452,21 +453,19 @@ theorem Term.freeVars_applySubst_subset (σ : Subst) (t a : Term)
     . contradiction
     next b heqb _ _ c heqc =>
     simp_all only [Term.signature]
-    have := Term.freeVars_applySubst_subset σ t₁ b heqb
-    have := Term.freeVars_applySubst_subset σ t₂ c heqc
+    have := Term.freeVars_applySubst_subset σ U t₁ b heqb
+    have := Term.freeVars_applySubst_subset σ U t₂ c heqc
     simp[Term.freeVars]
     all_goals
     simp at h₁
     rw[← h₁]
     simp[Term.freeVars]
     have := @Subst.freeVars_symbol_union σ t₁.signature t₂.signature
-    grind only [= Set.mem_union, = Set.subset_def]
+    grind only [= Set.subset_def, FCSet.to_set_diff, = Set.mem_union, = Set.mem_diff]
   | .applyFn f args =>
     match f with
     | .num n =>
-      simp[Term.applySubst, Option.bind] at h₁
-      split at h₁
-      . contradiction
+      simp[Term.applySubst] at h₁
       simp_all
     | .sym s =>
       simp_all only [Term.freeVars, Term.signature]
@@ -477,62 +476,66 @@ theorem Term.freeVars_applySubst_subset (σ : Subst) (t a : Term)
         split at h₁
         .
           simp at h₁
-          have := TermVector.freeVars_applySubst_subset σ args a' (by assumption)
-          have := Term.freeVars_applySubst_subset a'.toSubst (σ.get (Symbol.Function s)) a h₁
-          have := @toSubst.freeVars_inc _ a' (some (Term.signature (σ.get (Symbol.Function s))))
-          have := @Subst.freeVars_symbol_union σ (Function.signature (Fn.sym s)) args.signature
-          have := @Subst.free_vars_subset_fun σ s
-          grind only [= Set.mem_union, = Set.subset_def, FCSet.to_set_eq]
+          split at h₁
+          . contradiction
+          next _ heq =>
+            simp at h₁ heq
+            have := TermVector.freeVars_applySubst_subset σ U args a' (by assumption)
+            have := Term.freeVars_applySubst_subset a'.toSubst ∅ (σ.get (Symbol.Function s)) a h₁
+            have := @toSubst.freeVars_inc _ a' (some (Term.signature (σ.get (Symbol.Function s))))
+            have := @Subst.freeVars_symbol_union σ (Function.signature (Fn.sym s)) args.signature
+            have := @Subst.free_vars_subset_fun σ s
+            simp_all only [←Set.disjoint_iff_inter_eq_empty]
+            grind only [= Set.disjoint_left, = Set.subset_def, FCSet.to_set_diff,
+              = Set.mem_union, = Set.mem_diff]
         .
           simp at h₁
           rw[← h₁]
           simp[Term.freeVars]
-          have := TermVector.freeVars_applySubst_subset σ args a' (by assumption)
+          have := TermVector.freeVars_applySubst_subset σ U args a' (by assumption)
           have := @Subst.freeVars_symbol_union σ
-          grind only [= Set.mem_union, = Set.subset_def]
+          grind only [= Set.subset_def, FCSet.to_set_diff, = Set.mem_union, = Set.mem_diff]
 
   | .differential t =>
     simp[Term.applySubst, Option.bind] at h₁
     split at h₁
     . contradiction
     simp at h₁
-    split at h₁
-    . contradiction
-    next _ _ hg _ _ a' heq =>
-      simp at h₁ hg
+    next a' heq =>
       rw[←h₁]
       clear h₁
-      have := Term.freeVars_applySubst_subset σ _ _ heq
-      simp only [Term.freeVars, Finset.coe_union, Finset.coe_map, Term.signature]
-      grind only [= Set.mem_image, = Set.mem_empty_iff_false, = Set.mem_union, = Set.subset_def]
+      have := Term.freeVars_applySubst_subset σ .univ _ _ heq
+      simp only [Term.freeVars, Finset.coe_union, Finset.coe_map, Term.signature, FCSet.to_set_diff, FCSet.to_set_univ, Set.diff_univ, Set.union_empty] at *
+      grind only [= Set.mem_diff, = Set.mem_image, = Set.mem_union, = Set.subset_def]
 
 termination_by (σ.size, sizeOf t)
 decreasing_by
 all_goals simp_wf
 all_goals (try grind only [= Prod.lex_def])
-next hin =>
+next hin _ _ _ _ _ =>
   rw[TermVector.toSubst_size]
   apply Subst.symbol_size at hin
   grind only [= Prod.lex_def]
 end
 
 theorem Term.freeVars_applySubst_admissible_univ_subset (σ : Subst) (t a : Term)
-  : Term.applySubst σ t = some a
-  → σ.admissible FCSet.univ t.signature
+  : Term.applySubst σ FCSet.univ t = some a
   → (a.freeVars : Set Assignable ) ⊆ (t.freeVars : Set Assignable) := by
   intros h _
-  have := Term.freeVars_applySubst_subset σ t a h
-  simp_all only [FCSet.to_set_eq, FCSet.to_set_inter, FCSet.to_set_univ, Set.inter_univ,
-    FCSet.to_set_empty, Set.union_empty, Finset.coe_subset]
-
+  have := Term.freeVars_applySubst_subset σ FCSet.univ t a h
+  simp only [FCSet.to_set_diff, FCSet.to_set_univ, Set.diff_univ, Set.union_empty,
+    SetLike.coe_subset_coe, Finset.le_eq_subset] at this
+  apply this
 
 theorem Subst.preserve_semantics.term
   (σ : Subst)
+  (U : FCSet Assignable)
   (i : Interpretation)
-  (v : State)
+  (v w : State)
+  (hvw : v.isEqExcept w U)
   (t t' : Term)
-  (hs : t' = Term.applySubst σ t)
-  : Term.denote i v t' = Term.denote (Subst.adjoint σ i v) v t := by
+  (hs : t' = Term.applySubst σ U t)
+  : Term.denote i v t' = Term.denote (Subst.adjoint σ i w) v t := by
   match t with
     | .var x => simp_all[Term.applySubst, Term.denote]
     | .neg t =>
@@ -541,7 +544,7 @@ theorem Subst.preserve_semantics.term
       . contradiction
       .
         next a heq =>
-        have := Subst.preserve_semantics.term σ i v t a (by simp[heq])
+        have := Subst.preserve_semantics.term σ U i v w hvw t a (by simp[heq])
         simp_all[Term.denote]
     | .plus t₁ t₂
     | .times t₁ t₂ =>
@@ -554,15 +557,13 @@ theorem Subst.preserve_semantics.term
         . contradiction
         .
           next a ha _ _ b hb =>
-          have := Subst.preserve_semantics.term σ i v t₁ a (by simp[ha])
-          have := Subst.preserve_semantics.term σ i v t₂ b (by simp[hb])
+          have := Subst.preserve_semantics.term σ U i v w hvw t₁ a (by simp[ha])
+          have := Subst.preserve_semantics.term σ U i v w hvw t₂ b (by simp[hb])
           simp_all[Term.denote]
     | .applyFn f args =>
       match hf : f with
         | .num n =>
-          simp[Term.applySubst, Option.bind] at hs
-          split at hs
-          . contradiction
+          simp[Term.applySubst] at hs
           simp_all[Term.denote]
         | .sym s =>
           simp[Term.applySubst, Option.bind] at hs
@@ -570,41 +571,48 @@ theorem Subst.preserve_semantics.term
           .
             contradiction
           .
-            simp_all
+            simp at hs
             -- we do apply the subst
             split at hs
             next _ b _ _ =>
-
+              split at hs
+              . contradiction
+              simp_all
               simp[Term.denote]
 
               -- remove adjoint by Subst.preserve_semantics.termVector
               have : (fun (x : Fin s.arity) =>
-                        Term.denote (σ.adjoint i v) v args.toVector[↑(x : Nat)])
+                        Term.denote (σ.adjoint i w) v args.toVector[↑(x : Nat)])
                    = (fun (x : Fin s.arity) => Term.denote i v b.toVector[↑x]) := by
                     funext x
                     apply Eq.symm
-                    apply Subst.preserve_semantics.term
+                    apply Subst.preserve_semantics.term _ _ _ _ _ hvw
                     apply Eq.symm
                     apply Subst.apply_subst_term_vector_to_term
                     assumption
               rw[this]
 
-              apply Subst.preserve_semantics.term b.toSubst at hs
-              rw[hs]
-              rw[subst_adjoint_of_term_vector_to_subst]
-              simp only [adjoint]
-
+              apply Subst.preserve_semantics.term b.toSubst _ _ v v at hs
+              .
+                rw[hs]
+                rw[subst_adjoint_of_term_vector_to_subst]
+                simp only [adjoint]
+                apply Term.coincidence
+                simp_all[State.isEqExcept, ←Set.disjoint_iff_inter_eq_empty]
+                grind only [= Set.disjoint_left, Set.EqOn, = Set.mem_compl_iff]
+              .
+                simp_all only [State.isEqExcept, FCSet.to_set_empty, Set.compl_empty, Set.eqOn_univ]
             next a _ _ =>
               -- we don't apply subst
               simp_all
 
               -- remove adjoint by Subst.preserve_semantics.termVector
               have : (fun (x : Fin s.arity) =>
-                        Term.denote (σ.adjoint i v) v args.toVector[↑(x : ℕ)])
+                        Term.denote (σ.adjoint i w) v args.toVector[↑(x : ℕ)])
                    = (fun (x : Fin s.arity) => Term.denote i v a.toVector[↑x]) := by
                     funext x
                     apply Eq.symm
-                    apply Subst.preserve_semantics.term
+                    apply Subst.preserve_semantics.term _ _ _ _ _ hvw
                     apply Eq.symm
                     apply Subst.apply_subst_term_vector_to_term
                     assumption
@@ -612,18 +620,15 @@ theorem Subst.preserve_semantics.term
               simp[Term.denote]
               rw[this]
 
-              -- remove remaining adjoint because `σ.adjoint i v f = i f` if `f ∉ σ`
-              have := @Subst.adjoint_noeffect_nomem_fun i v s σ (by assumption)
+              -- remove remaining adjoint because `σ.adjoint i w f = i f` if `f ∉ σ`
+              have := @Subst.adjoint_noeffect_nomem_fun i w s σ (by assumption)
               rw[this]
               simp
     | .differential t =>
       simp[Term.applySubst, Option.bind] at hs
       split at hs
       . contradiction
-      simp at hs
-      split at hs
-      . contradiction
-      next _ _ hg _ _ a heq =>
+      next a heq =>
       simp at hs
       cases hs
       simp[Term.denote]
@@ -652,7 +657,7 @@ theorem Subst.preserve_semantics.term
       -- and hence substitution can *only reduce* free variables, e.g. {f(⋅) → 2}
       have : a.freeVars ⊆ t.freeVars := by
         have ih := Term.freeVars_applySubst_admissible_univ_subset
-              (σ := σ) t a heq (by simp_all[Subst.admissible])
+              (σ := σ) t a heq
         intro x hx
         have := ih hx
         grind
@@ -669,14 +674,10 @@ theorem Subst.preserve_semantics.term
       funext x
       congr
       funext y
-      have := by
-        apply @Subst.admissible_adjoint.term v (v.update x y) (v.update x y) σ i t FCSet.univ
-        . simp_all[Subst.admissible, Option.guard_eq_some']
-        . simp_all[State.isEqOn]
-      rw[this]
+      apply Subst.preserve_semantics.term _ FCSet.univ
+      . simp only [FCSet.to_set_univ, State.eq_except_univ]
+      . simp_all only
 
-      apply Subst.preserve_semantics.term σ i (v.update x y)
-      grind
 termination_by
   (σ.size, sizeOf t)
 decreasing_by
@@ -703,12 +704,12 @@ lemma ode_mapM_assignables_eq
   {σ : Subst}
   {system : OdeSystem}
   {ssystem : OdeSystem}
-  (h : system.mapM (fun x => do return ODE.mk x.var (← Term.applySubst σ x.term))
+  (h : system.mapM (fun x => do return ODE.mk x.var (← Term.applySubst σ ∅ x.term))
        = some ssystem)
   : OdeSystem.assignables ssystem = OdeSystem.assignables system := by
   unfold OdeSystem.assignables at *;
   induction system generalizing ssystem <;> simp_all +decide [ List.mapM_cons ];
-  cases h' : Term.applySubst σ ‹ODE›.term <;> simp_all +decide [ Option.bind_eq_some_iff ];
+  cases h' : Term.applySubst σ ∅ ‹ODE›.term <;> simp_all +decide [ Option.bind_eq_some_iff ];
   aesop
 
 lemma ode_evolution_formula_applySubst
@@ -716,7 +717,7 @@ lemma ode_evolution_formula_applySubst
   {system ssystem : OdeSystem}
   {Ψ Ψ' : Formula}
   : Formula.applySubst σ Ψ = some Ψ'
-  → system.mapM (fun x => do return ODE.mk x.var (← Term.applySubst σ x.term)) = some ssystem
+  → system.mapM (fun x => do return ODE.mk x.var (← Term.applySubst σ ∅ x.term)) = some ssystem
   → Formula.applySubst σ (odeEvolutionFormula system Ψ)
   = some (odeEvolutionFormula ssystem Ψ') := by
 
@@ -724,7 +725,7 @@ lemma ode_evolution_formula_applySubst
   induction system generalizing ssystem Ψ Ψ' with
     | nil => simp_all[odeEvolutionFormula]
     | cons head tail ih =>
-      cases _ : Term.applySubst σ head.term
+      cases _ : Term.applySubst σ ∅ head.term
       . simp_all
       .
         simp_all[Option.bind_eq_some_iff]
@@ -782,8 +783,8 @@ theorem Subst.preserve_semantics.formula
         split at hs
         . contradiction
         simp_all[Formula.denote]
-        have := Subst.preserve_semantics.term σ i v t₁
-        have := Subst.preserve_semantics.term σ i v t₂
+        have := Subst.preserve_semantics.term σ ∅ i v _ (Set.eqOn_refl _ _) t₁
+        have := Subst.preserve_semantics.term σ ∅ i v _ (Set.eqOn_refl _ _) t₂
         grind
       | .not Φ =>
         simp_all[Formula.denote, Formula.applySubst, Option.bind]
@@ -943,7 +944,7 @@ theorem Subst.preserve_semantics.formula
              = (fun (x : Fin p.arity) => Term.denote i v args'.toVector[↑x]) := by
                   funext x
                   apply Eq.symm
-                  apply Subst.preserve_semantics.term
+                  apply Subst.preserve_semantics.term _ ∅ _ _ _ (Set.eqOn_refl _ _)
                   apply Eq.symm
                   apply Subst.apply_subst_term_vector_to_term
                   assumption
@@ -990,7 +991,7 @@ theorem Subst.preserve_semantics.program
         . contradiction
         rename Term => t'
         simp_all[Program.denote]
-        have := Subst.preserve_semantics.term σ i v t t'
+        have := Subst.preserve_semantics.term σ ∅ i v _ (Set.eqOn_refl _ _) t t'
         grind
       | .random x =>
         simp[Program.applySubst] at hs
